remove duplicate code from NewPipeline.v, and sketch compiler_correct
combining upper and lower pipeline

compiler/src/compiler/NewPipeline.v
@@ -49,23 +49,12 @@ Require Import FunctionalExtensionality.
 Require Import coqutil.Tactics.autoforward.
 Require Import compiler.FitsStack.
 Require Import compiler.UpperPipeline.
+Require Import compiler.LowerPipeline.
 Import Utility.
 
 Existing Instance riscv.Spec.Machine.DefaultRiscvState.
 
 Open Scope Z_scope.
-
-Section WithWordAndMem.
-  Context {width: Z} {word: word.word width} {mem: map.map word byte}.
-
-  (* bedrock2.ptsto_bytes.ptsto_bytes takes an n-tuple of bytes, whereas this one takes a list of bytes *)
-  Definition ptsto_bytes: word -> list byte -> mem -> Prop := array ptsto (word.of_Z 1).
-
-  Definition mem_available(start pastend: word) : mem -> Prop :=
-    ex1 (fun anybytes: list byte =>
-      emp (Z.of_nat (List.length anybytes) = word.unsigned (word.sub pastend start)) *
-      (ptsto_bytes start anybytes))%sep.
-End WithWordAndMem.
 
 Module Import Pipeline.
 
@@ -151,415 +140,16 @@ Section Pipeline1.
   Local Notation flat_env := (@string_keyed_map p (list string * list string * FlatImp.stmt string)).
   Local Notation renamed_env := (@string_keyed_map p (list Z * list Z * FlatImp.stmt Z)).
 
-  Definition flattenPhase(prog: source_env): option flat_env := flatten_functions (2^10) prog.
-  Definition renamePhase(prog: flat_env): option renamed_env :=
-    rename_functions_new prog.
-  Definition spillingPhase(prog: renamed_env): option renamed_env := spill_functions prog.
-
-  (* Note: we could also track code size from the source program all the way to the target
-     program, and a lot of infrastructure is already there, will do once/if we want to get
-     a total compiler.
-     Returns the fun_pos_env so that users know where to jump to call the compiled functions. *)
-  Definition riscvPhase(prog: renamed_env):
-    option (list Instruction * funname_env Z * Z) :=
-    bind_opt stack_words_needed <- stack_usage prog;
-    let positions := FlatToRiscvDef.build_fun_pos_env prog in
-    let '(i, _) := FlatToRiscvDef.compile_funs positions prog in
-    Some (i, positions, stack_words_needed).
-
-  Definition composePhases{A B C: Type}(phase1: A -> option B)(phase2: B -> option C)(a: A) :=
-    match phase1 a with
-    | Some b => phase2 b
+  Definition composed_compile(functions: source_env): option (list Instruction * funname_env Z * Z) :=
+    match upper_compiler ext_spec width_cases functions with
+    | Some functions' => riscvPhase functions'
     | None => None
     end.
 
-  Definition composed_compile: source_env -> option (list Instruction * funname_env Z * Z) :=
-    composePhases (composePhases flattenPhase (composePhases renamePhase spillingPhase)) riscvPhase.
-
-  Definition FlatState(varname: Type){pp : FlatImp.parameters varname}: Type :=
-    FlatImp.env * FlatImp.stmt varname * bool * FlatImp.trace * FlatImp.mem * FlatImp.locals * MetricLog.
-
-  Definition flatExec{varname: Type}{pp : FlatImp.parameters varname}:
-    FlatState varname -> (FlatState varname -> Prop) -> Prop :=
-    fun '(e, s, done, t, m, l, mc) post =>
-      done = false /\
-      FlatImp.exec e s t m l mc (fun t' m' l' mc' => post (e, s, true, t', m', l', mc')).
-
-  (* Note: contrary to GhostConsts, this record only contains risc-v-related types, no FlatImp-related types *)
-  Record RiscvFrame: Type := {
-    addr_functions: word;
-    insts_functions: list Instruction;
-    stack_start: word;
-    stack_pastend: word;
-    xframe: mem -> Prop;
-    dframe: mem -> Prop;
-  }.
-
-  Definition satisfiesRiscvFrame(f: RiscvFrame)(mH: mem)(mach: MetricRiscvMachine): Prop :=
-      (program iset f.(addr_functions) f.(insts_functions) *
-       mem_available f.(stack_start) f.(stack_pastend) *
-       f.(dframe) * f.(xframe) * eq mH
-      )%sep mach.(getMem) /\
-      subset (footpr (program iset f.(addr_functions) f.(insts_functions) *
-                      f.(xframe))%sep)
-             (of_list (getXAddrs mach)) /\
-      word.unsigned (mach.(getPc)) mod 4 = 0 /\
-      mach.(getNextPc) = word.add mach.(getPc) (word.of_Z 4) /\
-      regs_initialized mach.(getRegs) /\
-      map.get mach.(getRegs) RegisterNames.sp = Some f.(stack_pastend) /\
-      (* configured by PrimitivesParams, can contain invariants needed for external calls *)
-      valid_machine mach.
-
   Local Instance map_ok': @map.ok (@word (@W p)) Init.Byte.byte (@mem p) := mem_ok.
-
-  Lemma get_build_fun_pos_env: forall e f,
-      map.get e f <> None ->
-      exists pos, map.get (FlatToRiscvDef.build_fun_pos_env e) f = Some pos.
-  Proof.
-    intros pos0 e.
-    unfold FlatToRiscvDef.build_fun_pos_env, FlatToRiscvDef.compile_funs.
-    eapply map.fold_spec.
-    - intros. rewrite map.get_empty in H. congruence.
-    - intros. destruct r as [ insts env]. simpl.
-      rewrite map.get_put_dec in H1.
-      rewrite map.get_put_dec.
-      destruct_one_match; eauto.
-  Qed.
-
-  Lemma get_compile_funs_pos: forall e,
-      let '(insts, posmap) := FlatToRiscvDef.compile_funs map.empty e in
-      forall f impl, map.get e f = Some impl -> exists pos2, map.get posmap f = Some pos2 /\ pos2 mod 4 = 0.
-  Proof.
-    intros e.
-    unfold FlatToRiscvDef.compile_funs.
-    eapply map.fold_spec.
-    - intros. rewrite map.get_empty in H. congruence.
-    - intros. destruct r as [ insts env]. simpl.
-      intros.
-      rewrite map.get_put_dec in H1.
-      rewrite map.get_put_dec.
-      destruct_one_match; eauto.
-      eexists. split; [reflexivity|].
-      solve_divisibleBy4.
-  Qed.
 
   Axiom TODO: False.
 
-  Lemma flatToRiscv_correct: forall functions pos_map stack_words_needed f_entry_name fbody instrs,
-      (forall f fun_impl, map.get functions f = Some fun_impl -> FlatToRiscvDef.valid_FlatImp_fun fun_impl) ->
-      riscvPhase functions = Some (instrs, pos_map, stack_words_needed) ->
-      map.get functions f_entry_name = Some (nil, nil, fbody) ->
-      exists f_entry_rel_pos,
-        map.get pos_map f_entry_name = Some f_entry_rel_pos /\
-        forall initial f mH mc postH retaddr,
-          instrs = f.(insts_functions) ->
-          satisfiesRiscvFrame f mH initial ->
-          initial.(getPc) = word.add f.(addr_functions) (word.of_Z f_entry_rel_pos) ->
-          map.get initial.(getRegs) RegisterNames.ra = Some retaddr ->
-          (* TODO probably better to execute
-             let c := SSeq SSkip (SCall nil f_entry_name nil) in
-             instead of fbody because otherwise we need to reprove all of the function's register saving code *)
-          FlatImp.exec functions fbody initial.(getLog) mH map.empty mc (fun t' m' l' mc' => postH t' m') ->
-          runsTo initial (fun final => exists mH',
-            postH final.(getLog) mH' /\
-            satisfiesRiscvFrame f mH' initial /\
-            final.(getPc) = retaddr).
-  Proof.
-    unfold riscvPhase. intros. simp.
-    edestruct get_build_fun_pos_env as (f_entry_rel_pos & GP). {
-      rewrite H1. discriminate.
-    }
-    eexists. split. 1: exact GP.
-    unfold satisfiesRiscvFrame.
-    intros. destruct_RiscvMachine initial. simp.
-    eapply runsTo_weaken.
-    - specialize compile_stmt_correct with (1 := @compile_ext_call_correct _ h).
-      unfold compiles_FlatToRiscv_correctly. intros compile_stmt_correct.
-      eapply compile_stmt_correct with (g := {| e_pos := (FlatToRiscvDef.build_fun_pos_env functions) |});
-        cbn; clear compile_stmt_correct.
-      1: eassumption.
-      3: eapply stack_usage_correct; eassumption.
-      { unfold map.extends. intros *. intro G.
-        rewrite map.get_remove_dec in G. destruct_one_match_hyp. 1: discriminate. exact G. }
-      { unfold good_e_impl.
-        intros *. intro G.
-        erewrite @map.get_remove_dec in G. 2,3: cbn; typeclasses eauto.
-        destruct_one_match_hyp. 1: discriminate.
-        split.
-        - eapply H. eassumption.
-        - unfold FlatToRiscvDef.build_fun_pos_env, FlatToRiscvDef.build_fun_pos_env.
-          pose proof (get_compile_funs_pos functions) as P.
-          destruct (FlatToRiscvDef.compile_funs map.empty functions) as [ insts posmap ] eqn: F.
-          eapply P.
-          eassumption. }
-      { reflexivity. }
-      { case TODO. (* FlatToRiscvDef.stmt_not_too_big *) }
-      { case TODO. (* FlatToRiscvDef.valid_FlatImp_vars fbody *) }
-      5: {
-        unfold goodMachine. cbn. ssplit.
-
-        (* TODO much more... *)
-  Admitted.
-
-  Lemma mem_available_to_exists: forall start pastend (m: mem) P,
-      (mem_available start pastend * P)%sep m ->
-      exists anybytes,
-        Z.of_nat (List.length anybytes) = word.unsigned (word.sub pastend start) /\
-        (ptsto_bytes start anybytes * P)%sep m.
-  Proof.
-    unfold mem_available. intros * H.
-    eapply sep_ex1_l in H. (* semicolon here fails *) destruct H.
-    eapply sep_assoc in H.
-    eapply sep_emp_l in H. destruct H.
-    eauto.
-  Qed.
-
-  Definition mem_to_available: forall start pastend (m: mem) P anybytes,
-     Z.of_nat (List.length anybytes) = word.unsigned (word.sub pastend start) ->
-     (ptsto_bytes start anybytes * P)%sep m ->
-     (mem_available start pastend * P)%sep m.
-  Proof.
-    unfold mem_available. intros * H Hsep.
-    eapply sep_ex1_l. eexists. eapply sep_assoc. eapply sep_emp_l. eauto.
-  Qed.
-
-  Lemma mod_2width_mod_bytes_per_word: forall x,
-      (x mod 2 ^ width) mod bytes_per_word = x mod bytes_per_word.
-  Proof.
-    intros.
-    rewrite <- Znumtheory.Zmod_div_mod.
-    - reflexivity.
-    - unfold bytes_per_word. destruct width_cases as [E | E]; rewrite E; reflexivity.
-    - destruct width_cases as [E | E]; rewrite E; reflexivity.
-    - unfold Z.divide.
-      exists (2 ^ width / bytes_per_word).
-      unfold bytes_per_word, Memory.bytes_per_word.
-      destruct width_cases as [E | E]; rewrite E; reflexivity.
-  Qed.
-
-  Lemma stack_length_divisible: forall (ml: MemoryLayout) {mlOk: MemoryLayoutOk ml},
-    word.unsigned (word.sub (MemoryLayout.stack_pastend ml) (MemoryLayout.stack_start ml)) mod bytes_per_word = 0.
-  Proof.
-    intros.
-    destruct mlOk.
-    rewrite word.unsigned_sub. unfold word.wrap.
-    rewrite mod_2width_mod_bytes_per_word.
-    rewrite Zminus_mod.
-    rewrite stack_start_aligned.
-    rewrite stack_pastend_aligned.
-    rewrite Z.sub_diag.
-    apply Zmod_0_l.
-  Qed.
-
-  Lemma program_mod_4_0: forall a instrs R m,
-      instrs <> [] ->
-      (program iset a instrs * R)%sep m ->
-      word.unsigned a mod 4 = 0.
-  Proof.
-    intros.
-    destruct instrs as [|instr instrs]. 1: congruence.
-    simpl in *.
-    unfold sep, ptsto_instr, sep, emp in *.
-    simp.
-    assumption.
-  Qed.
-
-  Lemma compile_funs_nonnil: forall e positions positions' f impl instrs,
-      map.get e f = Some impl ->
-      FlatToRiscvDef.compile_funs positions e = (instrs, positions') ->
-      instrs <> [].
-  Proof.
-    intros e positions.
-    unfold FlatToRiscvDef.compile_funs.
-    eapply map.fold_spec; intros.
-    - rewrite map.get_empty in H.
-      discriminate.
-    - rewrite map.get_put_dec in H1.
-      destr (k =? f)%string.
-      + subst.
-        unfold FlatToRiscvDef.add_compiled_function in H2. simp.
-        unfold FlatToRiscvDef.compile_function.
-        destruct impl as [ [args res] body ].
-        intro C. destruct l; discriminate.
-      + specialize H0 with (1 := H1).
-        destruct r as [ instrs'' positions'' ].
-        specialize H0 with (1 := eq_refl).
-        intro C. subst instrs.
-        unfold FlatToRiscvDef.add_compiled_function in H2. simp.
-        unfold FlatToRiscvDef.compile_function in *.
-        destruct v as [ [args res] body ].
-        destruct instrs''; discriminate.
-  Qed.
-
-  Ltac ignore_positions :=
-    repeat match goal with
-           | |- _ => reflexivity
-           | |- _ => rewrite !List.app_length
-           | |- _ => solve [eauto]
-           | |- _ => progress simpl
-           | |- S _ = S _ => f_equal
-           | |- (_ + _)%nat = (_ + _)%nat => f_equal
-           end.
-
-  Lemma compile_stmt_length_ignores_positions: forall posmap1 posmap2 c stackoffset pos1 pos2,
-      List.length (FlatToRiscvDef.compile_stmt posmap1 pos1 stackoffset c) =
-      List.length (FlatToRiscvDef.compile_stmt posmap2 pos2 stackoffset c).
-  Proof.
-    induction c; intros; ignore_positions.
-    apply compile_ext_call_length_ignores_positions.
-  Qed.
-
-  Lemma compile_function_length_ignores_positions: forall posmap1 posmap2 pos1 pos2 impl,
-      List.length (FlatToRiscvDef.compile_function posmap1 pos1 impl) =
-      List.length (FlatToRiscvDef.compile_function posmap2 pos2 impl).
-  Proof.
-    intros. destruct impl as [ [args rets] body ]. ignore_positions.
-    apply compile_stmt_length_ignores_positions.
-  Qed.
-
-  Lemma build_fun_pos_env_ignores_posmap_aux: forall posmap1 posmap2 e i1 m1 i2 m2,
-      map.fold (FlatToRiscvDef.add_compiled_function posmap1) ([], map.empty) e = (i1, m1) ->
-      map.fold (FlatToRiscvDef.add_compiled_function posmap2) ([], map.empty) e = (i2, m2) ->
-      m1 = m2 /\ List.length i1 = List.length i2.
-  Proof.
-    intros until e.
-    eapply map.fold_parametricity with (fa := (FlatToRiscvDef.add_compiled_function posmap1))
-                                       (fb := (FlatToRiscvDef.add_compiled_function posmap2));
-      intros.
-    - destruct a as [insts1 map1]. destruct b as [insts2 map2].
-      unfold FlatToRiscvDef.add_compiled_function in *.
-      inversion H0. inversion H1. subst. clear H0 H1.
-      specialize H with (1 := eq_refl) (2 := eq_refl). destruct H.
-      rewrite ?H0. subst.
-      split. 1: reflexivity.
-      ignore_positions.
-      apply compile_function_length_ignores_positions.
-    - inversion H. inversion H0. subst. auto.
-  Qed.
-
-  Lemma build_fun_pos_env_ignores_posmap: forall posmap1 posmap2 e,
-      snd (map.fold (FlatToRiscvDef.add_compiled_function posmap1) ([], map.empty) e) =
-      snd (map.fold (FlatToRiscvDef.add_compiled_function posmap2) ([], map.empty) e).
-  Proof.
-    intros.
-    destr (map.fold (FlatToRiscvDef.add_compiled_function posmap1) ([], map.empty) e).
-    destr (map.fold (FlatToRiscvDef.add_compiled_function posmap2) ([], map.empty) e).
-    simpl.
-    edestruct build_fun_pos_env_ignores_posmap_aux.
-    - exact E.
-    - exact E0.
-    - assumption.
-  Qed.
-
-  (* This lemma should relate two map.folds which fold two different f over the same env e:
-     1) FlatToRiscvDef.compile_funs, which folds FlatToRiscvDef.add_compiled_function.
-        Note that this one is called twice: First in build_fun_pos_env, and then in
-        compile_funs, and we rely on the order being the same both times.
-     2) functions, which folds sep
-     Note that 1) is not commutative (the iteration order determines in which order code
-     is layed out in memory), while 2) should be commutative because the "function"
-     separation logic predicate it seps onto the separation logic formula is the same
-     if we pass it the same function position map. *)
-  Lemma functions_to_program: forall functions_start e instrs pos_map stack_size,
-      riscvPhase e = Some (instrs, pos_map, stack_size) ->
-      iff1 (program iset functions_start instrs)
-           (FlatToRiscvCommon.functions functions_start (FlatToRiscvDef.build_fun_pos_env e) e).
-  Proof.
-    (* PARAMRECORDS *)
-    assert (map.ok FlatImp.env). { unfold FlatImp.env. simpl. typeclasses eauto. }
-    assert (map.ok mem) as Ok by exact mem_ok.
-
-    unfold riscvPhase.
-    intros.
-    simp.
-    unfold FlatToRiscvDef.compile_funs, functions in *.
-    remember (FlatToRiscvDef.build_fun_pos_env e) as positions.
-    (* choose your IH carefully! *)
-    lazymatch goal with
-    | |- ?G => enough ((forall f, map.get r f <> None <-> map.get e f <> None) /\
-                       ((forall f pos, map.get r f = Some pos -> map.get positions f = Some pos) -> G))
-    end.
-    1: {
-      destruct H0. apply H1; clear H1.
-      intros. rewrite <- H1. f_equal.
-      subst.
-      apply (f_equal snd) in E0. simpl in E0. rewrite <- E0.
-      transitivity (snd (map.fold (FlatToRiscvDef.add_compiled_function map.empty) ([], map.empty) e)).
-      - unfold FlatToRiscvDef.build_fun_pos_env, snd. reflexivity.
-      - apply build_fun_pos_env_ignores_posmap.
-    }
-    revert E0.
-    revert instrs r. clear E stack_size.
-    eapply (map.fold_spec (R:=(list Instruction * _))) with (m:=e); repeat (cbn || simp || intros).
-    { rewrite map.fold_empty. intuition try reflexivity.
-      - eapply H0. eapply map.get_empty.
-      - eapply H0. eapply map.get_empty.
-    }
-    rewrite map.fold_put; trivial.
-    2: { intros.
-      eapply functional_extensionality_dep; intros x.
-      eapply PropExtensionality.propositional_extensionality; revert x.
-      match goal with |- forall x, ?P x <-> ?Q x => change (iff1 P Q) end.
-      cancel. }
-    case r as (instrs'&r').
-    specialize H1 with (1 := eq_refl).
-    unfold FlatToRiscvDef.add_compiled_function in E0.
-    injection E0; clear E0; intros. subst.
-    unfold program in *.
-    wseplog_pre.
-    destruct H1.
-    split. {
-      intros. rewrite ?map.get_put_dec.
-      destr (k =? f)%string. 2: eauto. intuition discriminate.
-    }
-    intros.
-    rewrite H2. 2: {
-      intros.
-      eapply H3.
-      rewrite map.get_put_dec.
-      destr (k =? f)%string. 2: assumption.
-      subst. exfalso.
-      specialize (H1 f). unfold not in H1. rewrite H0 in H1. rewrite H4 in H1.
-      intuition congruence.
-    }
-    cancel.
-    unfold function.
-    specialize (H3 k).
-    rewrite map.get_put_same in H3.
-    specialize H3 with (1 := eq_refl).
-    simpl in *. rewrite H3.
-    cancel.
-    unfold program.
-    cancel_seps_at_indices 0%nat 0%nat. 2: reflexivity.
-    f_equal.
-    f_equal.
-    solve_word_eq word_ok.
-  Qed.
-
-  Definition machine_ok(p_functions: word)(f_entry_rel_pos: Z)(stack_start stack_pastend: word)
-             (finstrs: list Instruction)
-             (p_call pc: word)(mH: mem)(Rdata Rexec: mem -> Prop)(mach: MetricRiscvMachine): Prop :=
-      let CallInst := Jal RegisterNames.ra
-                          (f_entry_rel_pos + word.signed (word.sub p_functions p_call)) : Instruction in
-      (program iset p_functions finstrs *
-       program iset p_call [CallInst] *
-       mem_available stack_start stack_pastend *
-       Rdata * Rexec * eq mH
-      )%sep mach.(getMem) /\
-      subset (footpr (program iset p_functions finstrs *
-                      program iset p_call [CallInst] *
-                      Rexec)%sep)
-             (of_list (getXAddrs mach)) /\
-      word.unsigned (mach.(getPc)) mod 4 = 0 /\
-      mach.(getPc) = pc /\
-      mach.(getNextPc) = word.add mach.(getPc) (word.of_Z 4) /\
-      regs_initialized mach.(getRegs) /\
-      map.get mach.(getRegs) RegisterNames.sp = Some stack_pastend /\
-      (* configured by PrimitivesParams, can contain invariants needed for external calls *)
-      valid_machine mach.
-
-  (* This lemma translates "sim", which depends on the large definition "related", into something
-     more understandable and usable. *)
   Lemma compiler_correct: forall
       (ml: MemoryLayout)
       (mlOk: MemoryLayoutOk ml)
@@ -577,6 +167,7 @@ Section Pipeline1.
       composed_compile functions = Some (instrs, pos_map, required_stack_space) ->
       map.get functions f_entry_name = Some (nil, nil, fbody) ->
       map.get pos_map f_entry_name = Some f_entry_rel_pos ->
+      required_stack_space <= word.unsigned (word.sub (stack_pastend ml) (stack_start ml)) / bytes_per_word ->
       Semantics.exec functions fbody initial.(getLog) mH map.empty mc (fun t' m' l' mc' => postH t' m') ->
       machine_ok p_functions f_entry_rel_pos (MemoryLayout.stack_start ml) (MemoryLayout.stack_pastend ml)
                  instrs p_call p_call mH Rdata Rexec initial ->
@@ -585,21 +176,17 @@ Section Pipeline1.
           machine_ok p_functions f_entry_rel_pos (MemoryLayout.stack_start ml) (MemoryLayout.stack_pastend ml)
                      instrs p_call (word.add p_call (word.of_Z 4)) mH' Rdata Rexec final).
   Proof.
-    intros. unfold composed_compile in *. unfold composePhases at 1 in H0. simp.
-    unfold machine_ok in *. simp.
-    eapply runsTo_weaken.
-    - pose proof flatToRiscv_correct as P. specialize P with (2 := H0).
-      pose proof (upper_compiler_correct (Zlocals := locals)) as U. unfold phase_correct in U.
-      specialize U with (5 := E) (6 := H1). edestruct U as (fbody2 & G & Uc); clear U.
-      1-3: typeclasses eauto. 1: exact ext_spec_ok.
-      simp. specialize P with (2 := G). edestruct P as (fr & G' & Q); clear P.
-      { case TODO. (* FlatToRiscvDef.valid_FlatImp_fun fun_impl *) }
-      rewrite H2 in G'. apply Option.eq_of_eq_Some in G'. subst fr.
-      eapply Q with (f := {| addr_functions := p_functions |}); cbn; clear Q.
-      + reflexivity.
-      + unfold satisfiesRiscvFrame. cbn. case TODO.
-      +
-  Abort.
+    intros. unfold composed_compile in *. simp.
+    pose proof @upper_compiler_correct as U. unfold phase_correct in U.
+    specialize U with (Zlocals := locals) (5 := E) (6 := H1).
+    edestruct U as (fbody' & G' & Sim); clear U; try typeclasses eauto.
+    1: exact ext_spec_ok.
+    eapply @flat_to_riscv_correct; try typeclasses eauto; try eassumption.
+    { exact compile_ext_call_length_ignores_positions. }
+    { exact compile_ext_call_correct. }
+    { case TODO. (* something rename_fun_valid *) }
+    eapply Sim; clear Sim. eassumption.
+  Qed.
 
   Definition instrencode(p: list Instruction): list byte :=
     List.flat_map (fun inst => HList.tuple.to_list (LittleEndian.split 4 (encode inst))) p.
